Introducing the Indexed Monad Bitfield

specs/Memory.v
@@ -1,7 +1,10 @@
 Require Import FreeSpec.Libs.OpenNat.OpenNat.
 Require Import FreeSpec.PropBool.
-Require Import Coq.Program.Program.
+
 Require Import Coq.Arith.Arith.
+Require Import Coq.Program.Program.
+Require Import Coq.Setoids.Setoid.
+Require Import Omega.
 
 (** * Definitions
 
@@ -25,35 +28,93 @@ Definition qword := mem 64.
 Notation "x 'Byte'" := (x * 8) (at level 30, no associativity).
 Notation "x 'Bytes'" := (x * 8) (at level 30, no associativity).
 
+Definition mem_eq
+           {n: nat}
+           (m m': mem n)
+  : Prop :=
+  mem_val m = mem_val m'.
+
+Lemma mem_eq_refl
+      {n: nat}
+      (m: mem n)
+  : mem_eq m m.
+Proof.
+  reflexivity.
+Qed.
+
+Lemma mem_eq_sym
+      {n: nat}
+      (m m': mem n)
+  : mem_eq m m' -> mem_eq m' m.
+Proof.
+  intros.
+  symmetry.
+  exact H.
+Qed.
+
+Lemma mem_eq_trans
+      {n: nat}
+      (m m' m'': mem n)
+  : mem_eq m m'
+    -> mem_eq m' m''
+    -> mem_eq m m''.
+Proof.
+  intros H H'.
+  transitivity (mem_val m').
+  + exact H.
+  + exact H'.
+Qed.
+
+Add Parametric Relation
+    (n: nat)
+  : (mem n) (@mem_eq n)
+    reflexivity proved by mem_eq_refl
+    symmetry proved by mem_eq_sym
+    transitivity proved by mem_eq_trans
+      as mem_eq_rel.
+
 (** * Manipulation
 
     ** Boxing
 
  *)
-
 Program Definition box
         (n x: nat)
   : mem n :=
-  {| mem_val := x mod (2 ^ n)
+  {| mem_val := if lt_dec x (2 ^ n)
+                then x
+                else x mod (2 ^ n)
    ; mem_bound := _
    |}.
 Next Obligation.
-  apply Nat.mod_bound_pos.
-  + apply OpenNat.le_0_n.
-  + assert (G: forall z, 0 < 2 ^ z). {
-      clear x.
-      induction z.
-      + constructor.
-      + cbn.
-        rewrite OpenNat.add_0_r.
-        rewrite <- OpenNat.add_0_r at 1.
-        unfold lt.
-        rewrite <- OpenNat.add_succ_l.
-        apply OpenNat.add_le_mono.
-        ++ apply OpenNat.le_0_n.
-        ++ exact IHz.
-    }
-    exact (G n).
+  destruct (lt_dec  x (2 ^ n)).
+  + exact l.
+  + apply Nat.mod_bound_pos.
+    ++ apply OpenNat.le_0_n.
+    ++ assert (G: forall z, 0 < 2 ^ z). {
+         clear x n0.
+         induction z.
+         + constructor.
+         + cbn.
+           rewrite OpenNat.add_0_r.
+           rewrite <- OpenNat.add_0_r at 1.
+           unfold lt.
+           rewrite <- OpenNat.add_succ_l.
+           apply OpenNat.add_le_mono.
+           ++ apply OpenNat.le_0_n.
+           ++ exact IHz.
+       }
+       exact (G n).
+Defined.
+
+Add Parametric Morphism
+    (n: nat)
+  : (box n)
+    with signature (eq) ==> (@mem_eq n)
+      as box_morph.
+Proof.
+  intros y.
+  reflexivity.
 Defined.
 
 Definition zero
@@ -71,12 +132,57 @@ Definition unbox
   : nat :=
   mem_val x.
 
+Add Parametric Morphism
+    (n: nat)
+  : (@unbox n)
+    with signature (@mem_eq n) ==> eq
+      as unbox_morphism.
+Proof.
+  intros x y H.
+  unfold unbox.
+  rewrite H.
+  reflexivity.
+Defined.
+
 Definition cast
            {n: nat}
            (m: nat)
            (x: mem n)
   : mem m :=
   box m (unbox x).
+
+Add Parametric Morphism
+    (n: nat)
+    (m: nat)
+  : (@cast n m)
+    with signature (@mem_eq n) ==> eq
+      as cast_morphism.
+Proof.
+  intros x y H.
+  unfold cast.
+  rewrite H.
+  reflexivity.
+Defined.
+
+Lemma cast_same_size_eq
+      {n: nat}
+      (x: mem n)
+  : mem_eq (cast n x) x.
+Proof.
+  unfold cast.
+  unfold box.
+  unfold mem_eq.
+  cbn.
+  destruct lt_dec.
+  + unfold unbox.
+    reflexivity.
+  + assert (unbox x < 2 ^ n). {
+      unfold unbox.
+      apply (mem_bound x).
+    }
+    apply n0 in H.
+    destruct H.
+Qed.
 
 (** ** Arithmetic
 
@@ -88,6 +194,19 @@ Definition add
   : mem n :=
   box n (unbox x + unbox y).
 
+Add Parametric Morphism
+    (n: nat)
+  : (@add n)
+    with signature (@mem_eq n) ==> (@mem_eq n) ==> (@mem_eq n)
+      as add_morphism.
+Proof.
+  intros m m' H p p' H'.
+  unfold add.
+  rewrite H.
+  rewrite H'.
+  reflexivity.
+Defined.
+
 Definition shiftl
            {n: nat}
            (x: mem n)
@@ -95,12 +214,47 @@ Definition shiftl
   : mem n :=
     box n (Nat.shiftl (unbox x) b).
 
+Add Parametric Morphism
+    (n: nat)
+  : (@shiftl n)
+    with signature (@mem_eq n) ==> eq ==> (@mem_eq n)
+      as shiftl_morphism.
+Proof.
+  intros x y H z.
+  unfold shiftl.
+  rewrite H.
+  reflexivity.
+Defined.
+
 Definition shiftr
            {n: nat}
            (x: mem n)
            (b: nat)
   : mem n :=
     box n (Nat.shiftr (unbox x) b).
+
+Add Parametric Morphism
+    (n: nat)
+  : (@shiftr n)
+    with signature (@mem_eq n) ==> eq ==> (@mem_eq n)
+      as shiftr_morphism.
+Proof.
+  intros x y H z.
+  unfold shiftr.
+  rewrite H.
+  reflexivity.
+Defined.
+
+Lemma shiftr_0_eq
+      {n: nat}
+      (x: mem n)
+  : mem_eq (shiftr x 0) x.
+Proof.
+  unfold shiftr.
+  cbn.
+  fold (@cast n n x).
+  apply cast_same_size_eq.
+Qed.
 
 Definition mle
            {n: nat}
