specs/Bitfield.v
@@ -1,0 +1,183 @@
+Require Import Coq.Logic.FunctionalExtensionality.
+Require Import Coq.Logic.Eqdep.
+Require Import Coq.Program.Equality.
+
+Require Import FreeSpec.Control.
+Require Import FreeSpec.Control.Classes.
+Require Import FreeSpec.Control.Identity.
+Require Import FreeSpec.Control.State.
+Require Import FreeSpec.Specs.Memory.
+Require Import FreeSpec.WEq.
+
+Require Import Omega.
+
+(** * Definitions
+
+    We introduce the [Bitfield] _Indexed_ Monad. A computation of type
+    [Bitfield n A] will parse a [mem n] data and returns an [A]. Under
+    the hood, a [Bitfield m A] is a function which takes a natural
+    number and returns an element of [A].
+
+    ** The Indexed Monad
+
+ *)
+
+Definition Bitfield
+           (m: nat)
+           (A: Type)
+  := nat -> A.
+
+(** To actually perform the computation, that is parsing some kind of
+    memory to read the specified bitfield, the prefered way is to use
+    [parse]. It takes a [mem n] of the same size and return the parsed
+    bitfield..
+
+ *)
+
+Definition parse
+           {A: Type}
+           {n:  nat}
+           (bf: Bitfield n A)
+           (x:  mem n)
+  : A :=
+  bf (unbox x).
+
+(** ** Monadic Oprations
+
+    We define three monadic operations to use with the [Bitfield]
+    Indexed Monad:
+
+      - [bf_pure a] to create a [Bitfield 0] computation (parse nothing)
+        that always returns [a]
+      - [bf_bind p f] to bind two Bitfields together
+      - [field n] to parse a field of size [n]
+ *)
+
+Definition bf_pure
+           {A: Type}
+           (a: A)
+  : Bitfield 0 A :=
+  fun (n: nat)
+  => a.
+
+Definition bf_bind
+           {m m': nat}
+           {A B: Type}
+           (bf: Bitfield m A)
+           (f: A -> Bitfield m' B)
+  : Bitfield (m + m') B :=
+  fun (n: nat)
+  => (f (bf n)) (Nat.shiftr n m).
+
+Definition field
+        (m: nat)
+  : Bitfield m nat :=
+  fun (n: nat)
+  => n mod 2 ^ m.
+
+(** Indexed Monads are no Monad according to the definition of
+    [Monad]. Yet, the [Bitfield] computation has similar
+    properties. Therefore, we introduce similar notation.
+
+ *)
+
+Notation "p :>>= f" := (bf_bind p f)
+                         (at level 54).
+Notation "x :<- p ; q" := (p :>>= fun x => q)
+                            (at level 99, right associativity, p at next level).
+Notation "p :; q" := (p :>>= fun _ => q)
+                            (at level 99, right associativity).
+
+(** ** Additional Computations
+
+    These three oprations can be composed together. For instance, we
+    introduce the [skip] operation very easily.
+
+ *)
+
+Definition skip
+        (m: nat)
+  : Bitfield m unit :=
+  field m :;
+  bf_pure tt.
+
+Definition bit
+  : Bitfield 1 bool :=
+    x :<- field 1            ;
+    if Nat.eqb x 0
+    then bf_pure false
+    else bf_pure true.
+
+(** * Control Instances
+
+    Because [Bitfield] is indexed, it cannot be used easily with the
+    definition of the [FreeSpec.Control] library. However, the
+    [Bitfield] Indexed Monad should have similar properties and we now
+    prove these assertion.
+
+    We first define a very strong weak equality, because it is enough
+    for now. Maybe we will have to refine this latter.
+
+ *)
+
+(** ** Functor
+
+    For all [n], the [Bitfield n] computation _is_ a [Functor] and it
+    is pretty easy to show. Indeed, [Bitfield n] is actually a type
+    synonym for a plain function.
+
+ *)
+
+(** ** Applicative
+
+    To be an [Applicative] instance, a computation needs two
+    operation: [pure] and [apply]. The [pure] function of [Bitfield]
+    has been already defined: it is [bf_pure] (hence the name). As for
+    [apply], we define it now using [bf_bind] and our alternative
+    do-notation. Fortunately, this makes the implementation pretty
+    straightforward.
+
+ *)
+
+Definition bf_apply
+           {A B: Type}
+           {n m: nat}
+           (bff: Bitfield n (A -> B))
+           (bf: Bitfield m A)
+  : Bitfield (n + m) B :=
+  f :<- bff            ;
+  x :<- bf             ;
+  bf_pure (f x).
+
+(** The [Applicative] typeclass comes with several laws we need to
+    prove.
+
+ *)
+
+Fact bitfield_applicative_identity
+     {A: Type}
+     {m: nat}
+     (x: Bitfield m A)
+  : bf_apply (bf_pure id) x = x.
+Proof.
+  unfold bf_apply, bf_pure, bf_bind, id.
+  cbn.
+  reflexivity.
+Qed.
+
+(** * Examples
+
+ *)
+
+(* Here is an example (yet to be removed latter)
+ *)
+Definition SMRAMC_bf
+  : Bitfield 8 (bool * bool * bool) :=
+    skip 4                          :;
+    d_lck  :<- bit                   ;
+    d_cls  :<- bit                   ;
+    d_open :<- bit                   ;
+    skip 1                          :;
+    bf_pure (d_lck, d_cls, d_open)   .
+
+Eval vm_compute in (SMRAMC_bf 255).
